
投影矩阵

行向量下

对称的投影矩阵下有

$$
r = -l\\
t = -b\\
$$

$$
M = 
\begin{pmatrix}
\frac{n}{r} & 0 & 0 & 0\\
0 & \frac{n}{t} & 0 & 0\\
0 & 0 & \frac{-(f+n)}{f-n} & \frac{-2fn}{f-n}\\
0 & 0 & -1 & 0
\end{pmatrix}
$$

可以得到坐标的转化公式

$$
\begin{align*}
x_{clip} &= x_{view} \cdot \frac{n}{r}\\
y_{clip} &= y_{view} \cdot \frac{n}{t}\\
z_{clip} &= \frac{-(f+n)}{f-n} \cdot z_{view} + \frac{-2fn}{f-n}\\
w_{clip} &= -z_{view}   
\end{align*}
$$

$$
\begin{align*}
x_{ndc} = \frac{x_{clip}}{w_{clip}}\\
y_{ndc} = \frac{y_{clip}}{w_{clip}}\\
z_{ndc} = \frac{z_{clip}}{w_{clip}}\\
\end{align*}
$$

现在已知 $x_{ndc}， y_{ndc}， z_{view}$ 要求出$x_{view}， y_{view}$

记
$$
\begin{align*}
\frac{n}{r} = M_{00}\\
\frac{n}{t} = M_{11}\\
\frac{-(f+n)}{f-n} = M_{22}\\
\frac{-2fn}{f-n} = M_{23}\\
\end{align*}
$$

有

$$
\begin{align*}
x_{clip} &= x_{view} \cdot M_{00}\\
y_{clip} &= y_{view} \cdot M_{11}\\
z_{clip} &= z_{view} \cdot M_{22} + M_{23}\\
w_{clip} &= -z_{view}
\end{align*}
$$

$$
\begin{align*}
x_{view} &= \frac{x_{clip}}{M_{00}}\\
x_{clip} &= x_{ndc} \cdot w_{clip}\\
&= x_{ndc}  (-z_{view})\\
x_{view} &= \frac{- x_{ndc} \cdot z_{view}}{M_{00}}\\
\end{align*}
$$

同理

$$
y_{view} = \frac{- y_{ndc} \cdot z_{view}}{M_{11}}
$$