# 恒等变换

这里专门记录一些比较特别的恒等变换式子

常用的恒等变换式子


## 代数

$$
\begin{align*}
(y^2-y^{-2})^2 =& y^4 + y^{-4} -2\\
= &(y^2+y^{-2})^2 -4
\end{align*}
$$


$$
\dfrac{x^2}{1-x^2} = \dfrac{1}{2(1-x)} + \dfrac{1}{2(1+x)} -1
$$


### 代数恒等式


$$(a + b)^2 = a^2 + 2ab + b^2$$
$$(a - b)^2 = a^2 - 2ab + b^2$$
$$(ab)^2 = a^2 b^2$$
$$(a + b)^3 = a^3 + 3a^2b + 3ab^2 + b^3$$
$$(a - b)^3 = a^3 - 3a^2b + 3ab^2 - b^3$$
$$(a + b)(a - b) = a^2 - b^2$$
$$(a + b + c)^2 = a^2 + b^2 + c^2 + 2ab + 2bc + 2ca$$
$$a^3 + b^3 = (a + b)(a^2 - ab + b^2)$$
$$a^3 - b^3 = (a - b)(a^2 + ab + b^2)$$
$$(a + b)^2 - (a - b)^2 = 4ab$$
$$a^4 + b^4 = (a^2 + b^2)^2 - 2a^2b^2$$
$$a^4 - b^4 = (a^2 - b^2)(a^2 + b^2)$$
$$(a^2 + b^2)^2 = a^4 + 2a^2b^2 + b^4$$
$$(a + b + c)(a + b - c) = a^2 + 2ab + b^2 - c^2$$
$$a^3 + b^3 + c^3 - 3abc = (a + b + c)(a^2 + b^2 + c^2 - ab - bc - ca)$$
